src/dvspec/dafny/att_spec_proofs/ind_inv.dfy
@@ -5,11 +5,7 @@ include "../specification/consensus.dfy"
 include "../specification/network.dfy"
 include "../specification/dvn.dfy"
 include "../att_spec_proofs/inv.dfy"
-include "../att_spec_proofs/fnc_invs_1_26.dfy"
-include "../att_spec_proofs/fnc_invs_27.dfy"
 include "../att_spec_proofs/dvn_next_invs_1_7.dfy"
-include "../att_spec_proofs/dvn_next_invs_8_18.dfy"
-include "../att_spec_proofs/dvn_next_invs_19_26.dfy"
 include "common_proofs.dfy"
 
 module Att_Ind_Inv_With_Empty_Initial_Attestation_Slashing_DB
@@ -22,12 +18,8 @@ module Att_Ind_Inv_With_Empty_Initial_Attestation_Slashing_DB
     import opened DV    
     import opened Att_Inv_With_Empty_Initial_Attestation_Slashing_DB
     import opened Helper_Sets_Lemmas
-    import opened Fnc_Invs_1_26   
-    import opened Fnc_Invs_27   
     import opened Common_Proofs
     import opened DVN_Next_Invs_1_7
-    import opened DVN_Next_Invs_8_18
-    import opened DVN_Next_Invs_19_26
 
     lemma ConsensusSpec_Init_implies_inv41<D(!new, 0)>(dvn: DVState, ci: ConsensusInstance<D>)
     requires ConsensusSpec.Init(ci, dvn.all_nodes, dvn.honest_nodes_states.Keys)
